testdata/out/go/error_gk/error_gk.go
@@ -1,5 +1,7 @@
 package error_gk
 
+import "github.com/tchajed/marshal"
+
 type E uint32
 
 const (
@@ -7,6 +9,15 @@ const (
 	EEndOfFile E = 1
 	EUnknown   E = 2
 )
+
+func Marshal(enc []byte, e E) []byte {
+	return marshal.WriteInt32(enc, uint32(e))
+}
+
+func Unmarshal(s []byte) (E, []byte) {
+	e_raw, s := marshal.ReadInt32(s)
+	return E(e_raw), s
+}
 
 var Name = map[uint32]string{
 	0: "eOk",
